wip: backport labels into capture sets.

CaptureSets.v
@@ -12,6 +12,7 @@ Require Import FSetFacts.
 Require Import Atom.
 Require Import Nat.
 Require Export Bool.
+Require Import Label.
 
 Create HintDb csets.
 
@@ -23,7 +24,7 @@ Create HintDb csets.
     bound variables, and if we contain the special
     `universal` variable. *)
 Inductive cap : Type :=
-  | cset_set : atoms -> nats -> bool -> cap.
+  | cset_set : atoms -> nats -> bool -> labels -> cap.
 
 (** ************************************************** *)
 (** Constructors *)
@@ -31,27 +32,30 @@ Inductive cap : Type :=
 
 Declare Scope cset_shorthand.
 
-Notation "`cset_fvar` a" := (cset_set {a}A {}N false)
+Notation "`cset_fvar` a" := (cset_set {a}A {}N false {}L)
                               (at level 10, a at level 9) : cset_shorthand.
 
-Notation "`cset_bvar` k" := (cset_set {}A {k}N false)
+Notation "`cset_bvar` k" := (cset_set {}A {k}N false {}L)
                               (at level 10, k at level 9) : cset_shorthand.
 
-Notation "{}" := (cset_set {}A {}N false) : cset_shorthand.
-Notation "{*}" := (cset_set {}A {}N true) : cset_shorthand.
+Notation "{}" := (cset_set {}A {}N false {}L) : cset_shorthand.
+Notation "{*}" := (cset_set {}A {}N true {}L) : cset_shorthand.
 
 (** ************************************************** *)
 (** Selectors *)
 (** ************************************************** *)
 
-Notation "`cset_fvars` C" := (match C with cset_set xs _ _ => xs end)
-                               (at level 10, C at level 9) : cset_shorthand.
+Notation "`cset_fvars` C" := (match C with cset_set xs _ _ _ => xs end)
+                                (at level 10, C at level 9) : cset_shorthand.
 
-Notation "`cset_bvars` C" := (match C with cset_set _ ks _ => ks end)
-                               (at level 10, C at level 9) : cset_shorthand.
+Notation "`cset_bvars` C" := (match C with cset_set _ ks _ _ => ks end)
+                                (at level 10, C at level 9) : cset_shorthand.
 
-Notation "`cset_uvar` C" := (match C with cset_set _ _ u => u end)
-                               (at level 10, C at level 9) : cset_shorthand.
+Notation "`cset_uvar` C" := (match C with cset_set _ _ u _ => u end)
+                                (at level 10, C at level 9) : cset_shorthand.
+
+Notation "`cset_lvars` C" := (match C with cset_set _ _ _ l => l end)
+                                (at level 10, C at level 9) : cset_shorthand.
 
 (** ************************************************** *)
 (** Operations *)
@@ -72,31 +76,42 @@ Definition cset_union (c1 c2 : cap) : cap :=
   cset_set
     (AtomSet.F.union (`cset_fvars` c1) (`cset_fvars` c2))
     (NatSet.F.union (`cset_bvars` c1) (`cset_bvars` c2))
-    ((`cset_uvar` c1) || (`cset_uvar` c2)).
+    ((`cset_uvar` c1) || (`cset_uvar` c2))
+    (LabelSet.F.union (`cset_lvars` c1) (`cset_lvars` c2)).
 
 Definition cset_subset_dec (C D : cap) :=
   AtomSet.F.subset (`cset_fvars` C) (`cset_fvars` D)
     && NatSet.F.subset (`cset_bvars` C) (`cset_bvars` D)
-    && (implb (`cset_uvar` C) (`cset_uvar` D)).
+    && (implb (`cset_uvar` C) (`cset_uvar` D))
+    && LabelSet.F.subset (`cset_lvars` C) (`cset_lvars` D).
 
 Notation "C `u` D" := (cset_union C D) (at level 69) : cset_shorthand.
-Notation "C A`\` x" := (cset_set ((`cset_fvars` C) `\`A x) (`cset_bvars` C) (`cset_uvar` C))
+Notation "C A`\` x" := (cset_set ((`cset_fvars` C) `\`A x) (`cset_bvars` C) (`cset_uvar` C) (`cset_lvars` C))
                          (at level 69) : cset_shorthand.
 Notation "x A`in` C" := (AtomSet.F.In x (`cset_fvars` C))
                           (at level 69) : cset_shorthand.
 Notation "x A`mem` C" := (AtomSet.F.mem x (`cset_fvars` C)) (at level 69) : cset_shorthand.
 
-Notation "C N`\` k" := (cset_set ((`cset_fvars` C) ) ((`cset_bvars` C) `\`N k) (`cset_uvar` C))
+Notation "C N`\` k" := (cset_set ((`cset_fvars` C) ) ((`cset_bvars` C) `\`N k) (`cset_uvar` C) (`cset_lvars` C))
                          (at level 69) : cset_shorthand.
 Notation "k N`in` C" := (NatSet.F.In k (`cset_bvars` C))
                           (at level 69) : cset_shorthand.
 Notation "k N`mem` C" := (NatSet.F.mem k (`cset_bvars` C))
                            (at level 69) : cset_shorthand.
+                      
+
+Notation "C L`\` k" := (cset_set ((`cset_fvars` C) ) ((`cset_bvars` C)) ((`cset_uvar` C)) ((`cset_lvars` C) `\`L k))
+                          (at level 69) : cset_shorthand.
+Notation "k L`in` C" := (LabelSet.F.In k (`cset_lvars` C))
+                            (at level 69) : cset_shorthand.
+Notation "k L`mem` C" := (LabelSet.F.mem k (`cset_lvars` C))
+                            (at level 69) : cset_shorthand.
 
 Notation "`* mem` C" := (`cset_uvar` C)
                            (at level 10, only parsing) : cset_shorthand.
 Notation "`* in` C" := (`cset_uvar` C = true)
                            (at level 10) : cset_shorthand.
+                  
 
 
 Notation "`cset_references_bvar` k c" :=
@@ -126,6 +141,16 @@ Notation "`cset_references_univ` c" :=
   (`* in` c)
     (at level 10, only parsing) : cset_shorthand.
 
+Notation "`cset_references_lvar` a c" :=
+  (a L`in` c)
+    (at level 10, a at level 9, c at level 9, only parsing) : cset_shorthand.
+Notation "`cset_references_lvar_dec` a c" :=
+  (a L`mem` c)
+    (at level 10, a at level 9, c at level 9, only parsing) : cset_shorthand.
+Notation "`cset_remove_lvar` a c" :=
+  (c L`\` a)
+    (at level 10, a at level 9, c at level 9, only parsing) : cset_shorthand.
+    
 
 (* Check (fun x =>  fun N => x N`in` N). *)
 (* Check (fun C D x => (cset_union D (cset_remove_fvar x C))). *)
@@ -141,12 +166,13 @@ Notation "{ x 'as' N}" := (`cset_bvar` x) : experimental_set_scope.
 
 Definition cset_empty (c : cap) : Prop :=
   AtomSet.F.Empty (`cset_fvars` c) /\ NatSet.F.Empty (`cset_bvars` c) /\
-    ((`cset_uvar` c) = false).
+    ((`cset_uvar` c) = false) /\ LabelSet.F.Empty (`cset_lvars` c).
 
 Definition cset_subset_prop (c : cap) (d : cap) : Prop :=
   AtomSet.F.Subset (`cset_fvars` c) (`cset_fvars` d)
     /\ NatSet.F.Subset (`cset_bvars` c) (`cset_bvars` d)
-    /\  (leb (`cset_uvar` c) (`cset_uvar` d)).
+    /\  (leb (`cset_uvar` c) (`cset_uvar` d))
+    /\ LabelSet.F.Subset (`cset_lvars` c) (`cset_lvars` d).
 
 
 (** ************************************************** *)
@@ -160,6 +186,8 @@ Section Props.
   Variable k n : nat.
   Variable N N1 N2 : nats.
   Variable C D C1 C2 C3 : cap.
+  Variable x1 x2 x3 x4 : label.
+  Variable L X1 X2 X3 X4 : labels.
 
   Lemma cset_bvar_mem_iff :
     `cset_references_bvar` k C <-> `cset_references_bvar_dec` k C = true.
@@ -180,6 +208,13 @@ Section Props.
   Proof.
     destruct C;
     reflexivity.
+  Qed.
+
+  Lemma cset_lvar_mem_iff :
+    `cset_references_lvar` x1 C <-> `cset_references_lvar_dec` x1 C = true.
+  Proof.
+    destruct C ;
+      simpl in *; intuition.
   Qed.
 
   Lemma cset_bvar_not_mem_iff :
@@ -206,13 +241,22 @@ Section Props.
     intro; subst; auto.
   Qed.
 
-  Lemma fvars_1 : `cset_fvars` (cset_set A N R) = A.
+  Lemma cset_lvar_not_mem_iff :
+    ~ `cset_references_lvar` x1 C <-> `cset_references_lvar_dec` x1 C = false.
+  Proof.
+    destruct C ; rewrite <- LabelSetFacts.not_mem_iff; fnsetdec.
+  Qed.
+
+  Lemma fvars_1 : `cset_fvars` (cset_set A N R L) = A.
   Proof. trivial. Qed.
 
-  Lemma bvars_1 : `cset_bvars` (cset_set A N R) = N.
+  Lemma bvars_1 : `cset_bvars` (cset_set A N R L) = N.
   Proof. trivial. Qed.
 
-  Lemma lvars_1 : `cset_uvar` (cset_set A N R) = R.
+  Lemma uvars_1 : `cset_uvar` (cset_set A N R L) = R.
+  Proof. trivial. Qed.
+
+  Lemma lvars_1 : `cset_lvars` (cset_set A N R L) = L.
   Proof. trivial. Qed.
 
   Lemma fvars_union_1 : `cset_fvars` (cset_union C D) = AtomSet.F.union (`cset_fvars` C) (`cset_fvars` D).
@@ -221,13 +265,19 @@ Section Props.
   Lemma bvars_union_1 : `cset_bvars` (cset_union C D) = NatSet.F.union (`cset_bvars` C) (`cset_bvars` D).
   Proof. trivial. Qed.
 
-  Lemma lvars_union_1 : `cset_uvar` (cset_union C D) = orb (`cset_uvar` C) (`cset_uvar` D).
+  Lemma uvar_union_1 : `cset_uvar` (cset_union C D) = orb (`cset_uvar` C) (`cset_uvar` D).
+  Proof. trivial. Qed.
+  
+  Lemma lvars_union_1 : `cset_lvars` (cset_union C D) = LabelSet.F.union (`cset_lvars` C) (`cset_lvars` D).
   Proof. trivial. Qed.
 
-  Lemma remove_fvar_1 : `cset_remove_fvar` x (cset_set A N R) = (cset_set (AtomSet.F.remove x A) N R).
+  Lemma remove_fvar_1 : `cset_remove_fvar` x (cset_set A N R L) = (cset_set (AtomSet.F.remove x A) N R L).
   Proof. intros. simpl in *. trivial. Qed.
 
-  Lemma remove_bvar_1 : `cset_remove_bvar` k (cset_set A N R) = (cset_set A (NatSet.F.remove k N) R).
+  Lemma remove_bvar_1 : `cset_remove_bvar` k (cset_set A N R L) = (cset_set A (NatSet.F.remove k N) R L).
+  Proof. intros. simpl in *. trivial. Qed.
+
+  Lemma remove_lvar_1 : `cset_remove_lvar` x1 (cset_set A N R L) = (cset_set A N R (LabelSet.F.remove x1 L)).
   Proof. intros. simpl in *. trivial. Qed.
 
   Lemma mem_bvar_1 : `cset_references_bvar` k C -> `cset_references_bvar_dec` k C = true.
@@ -242,11 +292,17 @@ Section Props.
   Lemma mem_fvar_2 : `cset_references_fvar_dec` a C = true -> `cset_references_fvar` a C.
   Proof. rewrite <- cset_fvar_mem_iff; trivial. Qed.
 
-  Lemma mem_lvar_1 : `cset_references_univ` C -> `cset_references_univ_dec` C = true.
+  Lemma mem_uvar_1 : `cset_references_univ` C -> `cset_references_univ_dec` C = true.
   Proof. trivial. Qed.
 
-  Lemma mem_lvar_2 : `cset_references_univ_dec` C = true -> `cset_references_univ` C.
+  Lemma mem_uvar_2 : `cset_references_univ_dec` C = true -> `cset_references_univ` C.
   Proof. trivial. Qed.
+
+  Lemma mem_lvar_1 : `cset_references_lvar` x1 C -> `cset_references_lvar_dec` x1 C = true.
+  Proof. rewrite cset_lvar_mem_iff; trivial. Qed.
+
+  Lemma mem_lvar_2 : `cset_references_lvar_dec` x1 C = true -> `cset_references_lvar` x1 C.
+  Proof. rewrite <- cset_lvar_mem_iff; trivial. Qed.
 
   Lemma In_bvar_1 : k = n -> `cset_references_bvar` k C -> `cset_references_bvar` n C.
   Proof. intros; subst; trivial. Qed.
@@ -254,8 +310,11 @@ Section Props.
   Lemma In_fvar_1 : a = f -> `cset_references_fvar` a C -> `cset_references_fvar` f C.
   Proof. intros; subst; trivial. Qed.
 
+  Lemma In_lvar_1 : x1 = x2 -> `cset_references_lvar` x1 C -> `cset_references_lvar` x2 C.
+  Proof. intros; subst; trivial. Qed.
+
   Lemma Is_empty : cset_empty {}.
-  Proof. repeat split. fsetdec. fnsetdec. Qed.
+  Proof. repeat split. fsetdec. fnsetdec. lsetdec. Qed.
 
   Lemma union_fvar_1 : `cset_references_fvar` x (cset_union C D) -> `cset_references_fvar` x C \/ `cset_references_fvar` x D.
   Proof. intros. unfold cset_union in *; simpl in *. fsetdec. Qed.
@@ -275,19 +334,28 @@ Section Props.
   Lemma union_bvar_3 : `cset_references_bvar` k D -> `cset_references_bvar` k (cset_union C D).
   Proof. unfold cset_union in *; simpl in *. fnsetdec. Qed.
 
-  Lemma union_lvar_1 : `cset_references_univ` (cset_union C D) ->
+  Lemma union_uvar_1 : `cset_references_univ` (cset_union C D) ->
     `cset_references_univ` C \/ `cset_references_univ` D.
   Proof. intros. unfold cset_union in *; simpl in *.
     rewrite orb_true_iff in H; auto*.
   Qed.
 
-  Lemma union_lvar_2 : `cset_references_univ` C -> `cset_references_univ` (cset_union C D).
+  Lemma union_uvar_2 : `cset_references_univ` C -> `cset_references_univ` (cset_union C D).
   Proof. unfold cset_union in *; simpl in *. intro.
     rewrite orb_true_iff. auto. Qed.
 
-  Lemma union_lvar_3 : `cset_references_univ` D -> `cset_references_univ` (cset_union C D).
+  Lemma union_uvar_3 : `cset_references_univ` D -> `cset_references_univ` (cset_union C D).
   Proof. unfold cset_union in *; simpl in *. intro.
     rewrite orb_true_iff. auto. Qed.
+
+  Lemma union_lvar_1 : `cset_references_lvar` x1 (cset_union C D) -> `cset_references_lvar` x1 C \/ `cset_references_lvar` x1 D.
+  Proof. intros. unfold cset_union in *; simpl in *. lsetdec. Qed.
+
+  Lemma union_lvar_2 : `cset_references_lvar` x1 C -> `cset_references_lvar` x1 (cset_union C D).
+  Proof. unfold cset_union in *; simpl in *. lsetdec. Qed.
+
+  Lemma union_lvar_3 : `cset_references_lvar` x1 D -> `cset_references_lvar` x1 (cset_union C D).
+  Proof. unfold cset_union in *; simpl in *. lsetdec. Qed.
 
   Lemma union_sub_1 : cset_subset_prop C D -> cset_union D C = D.
   Proof.
@@ -295,6 +363,7 @@ Section Props.
     intros. destruct C; destruct D; simpl; f_equal.
     fsetdec. fnsetdec.
       destruct b; destruct b0; auto*.
+    lsetdec.
   Qed.
 
   Lemma union_sub_2 : cset_subset_prop C D -> D = cset_union D C.
@@ -303,13 +372,14 @@ Section Props.
     intros. destruct C; destruct D; simpl; f_equal.
     fsetdec. fnsetdec.
       destruct b; destruct b0; auto*.
+    lsetdec.
   Qed.
 
   Lemma union_subset_distribute_1 : cset_subset_prop C1 C2 -> cset_subset_prop (cset_union C1 D) (cset_union C2 D).
   Proof.
     intros. unfold cset_subset_prop in *; inversion H as [Sub_F [Sub_B Sub_A]];
     unfold cset_union in *; destruct C1; destruct C2.
-    repeat split; try fsetdec; try fnsetdec.
+    repeat split; try fsetdec; try fnsetdec; try lsetdec.
       destruct b; destruct b0; unfold leb in *; simpl in *; destruct D; destruct b; auto*.
   Qed.
 
@@ -330,15 +400,16 @@ Hint Rewrite
 
 
 Hint Resolve
-  mem_bvar_1 mem_fvar_1 Is_empty
+  mem_bvar_1 mem_fvar_1 mem_uvar_1 mem_lvar_1 Is_empty
   union_fvar_1 union_fvar_2 union_fvar_3
   union_bvar_1 union_bvar_2 union_bvar_3
+  union_uvar_1 union_uvar_2 union_uvar_3
   union_lvar_1 union_lvar_2 union_lvar_3
   union_sub_1 union_sub_2 union_subset_distribute_1
   subset_univ_1
 : core.
 
-Hint Immediate In_bvar_1 In_fvar_1 mem_bvar_2 mem_fvar_2 mem_lvar_2 : core.
+Hint Immediate In_bvar_1 In_fvar_1 mem_bvar_2 mem_fvar_2 mem_lvar_2 mem_uvar_2 : core.
 
 (* Some subset properties *)
 Lemma subset_refl : forall C,
@@ -346,6 +417,7 @@ Lemma subset_refl : forall C,
 Proof.
   intros. unfold cset_subset_prop. repeat split. fsetdec. fnsetdec.
     unfold leb; destruct C; destruct b; auto*.
+  lsetdec.
 Qed.
 
 Lemma subset_union_left : forall C1 C2,
@@ -354,6 +426,7 @@ Proof.
   intros. destruct C1. destruct C2. unfold cset_subset_prop, cset_union.
   repeat split. fsetdec. fnsetdec.
     destr_bool.
+  lsetdec.
 Qed.
 
 Lemma subset_union_right : forall C1 C2,
@@ -362,15 +435,16 @@ Proof.
   intros. destruct C1. destruct C2. unfold cset_subset_prop, cset_union.
   repeat split. fsetdec. fnsetdec.
     destr_bool.
+  lsetdec.
 Qed.
 
 Lemma subset_trans : forall A B C,
   cset_subset_prop A B -> cset_subset_prop B C -> cset_subset_prop A C.
 Proof.
   intros * AB BC.
-  inversion AB as [ABF [ABN ABL]]; subst; inversion BC as [BCF [BCN BCL]]; subst...
-  repeat (econstructor; try fsetdec; try fnsetdec)...
-  destruct A; destruct B; destruct C; destr_bool.
+  inversion AB as [ABF [ABN [ABU ABL]]]; subst; inversion BC as [BCF [BCN [BCU BCL]]]; subst...
+  repeat (econstructor; try fsetdec; try fnsetdec; try lsetdec)...
+  destruct A; destruct B; destruct C; destr_bool...
 Qed.
 
 Hint Immediate subset_union_left subset_union_right  subset_refl: core.
@@ -391,15 +465,19 @@ Ltac rewrite_set_facts_in H :=
   | NatSet.F.mem _ _ = false => rewrite <- NatSetFacts.not_mem_iff in H
   | AtomSet.F.mem _ _ = true => rewrite <- AtomSetFacts.mem_iff in H
   | AtomSet.F.mem _ _ = false => rewrite <- AtomSetFacts.not_mem_iff in H
+  | LabelSet.F.mem _ _ = true => rewrite <- LabelSetFacts.mem_iff in H
+  | LabelSet.F.mem _ _ = false => rewrite <- AtomSetFacts.not_mem_iff in H
   | `cset_references_bvar_dec` _ _ = true => rewrite <- cset_bvar_mem_iff in H
   | `cset_references_fvar_dec` _ _ = true => rewrite <- cset_fvar_mem_iff in H
   | `cset_references_univ_dec` _ _ = true => rewrite <- cset_univ_mem_iff in H
+  | `cset_references_lvar_dec` _ _ = true => rewrite <- cset_lvar_mem_iff in H
   | `cset_references_bvar_dec` _ _ = false => rewrite <- cset_bvar_not_mem_iff in H
   | `cset_references_fvar_dec` _ _ = false => rewrite <- cset_fvar_not_mem_iff in H
   | `cset_references_univ_dec` _ _ = false => rewrite <- cset_univ_not_mem_iff in H
+  | `cset_references_lvar_dec` _ _ = false => rewrite <- cset_lvar_not_mem_iff in H
   end;
   (** argh, unused arguments need to be discharged *)
-  try apply NatSet.F.empty; try apply AtomSet.F.empty; try apply {}.
+  try apply NatSet.F.empty; try apply AtomSet.F.empty; try apply LabelSet.F.empty; try apply {}.
 
 Ltac rewrite_set_facts_back_in H :=
   match type of H with
@@ -412,15 +490,19 @@ Ltac rewrite_set_facts_back_in H :=
   | (~ NatSet.F.In _ _)      => rewrite -> NatSetFacts.not_mem_iff in H
   | AtomSet.F.In _ _         => rewrite -> AtomSetFacts.mem_iff in H
   | (~ AtomSet.F.In _ _)     => rewrite -> AtomSetFacts.not_mem_iff in H
+  | LabelSet.F.In _ _        => rewrite -> LabelSetFacts.mem_iff in H
+  | (~ LabelSet.F.In _ _ )   => rewrite -> LabelSetFacts.mem_iff in H
   | `cset_references_bvar` _ _ => rewrite -> cset_bvar_mem_iff in H
   | `cset_references_fvar` _ _ => rewrite -> cset_fvar_mem_iff in H
   | `cset_references_univ` _ _ => rewrite -> cset_univ_mem_iff in H
+  | `cset_references_univ` _ _ => rewrite -> cset_lvar_mem_iff in H
   | (~ `cset_references_bvar` _ _) => rewrite -> cset_bvar_not_mem_iff in H
   | (~ `cset_references_fvar` _ _) => rewrite -> cset_fvar_not_mem_iff in H
   | (~ `cset_references_univ` _ _) => rewrite -> cset_univ_not_mem_iff in H
+  | (~ `cset_references_lvar` _ _) => rewrite -> cset_lvar_not_mem_iff in H
   end;
   (** argh, unused arguments need to be discharged *)
-  try apply NatSet.F.empty; try apply AtomSet.F.empty; try apply {}.
+  try apply NatSet.F.empty; try apply AtomSet.F.empty; try apply LabelSet.F.empty; try apply {}.
 
 Ltac simpl_in_cset :=
   let go H := rewrite_set_facts_back_in H; try rewrite H in *; rewrite_set_facts_in H in
@@ -432,6 +514,8 @@ Ltac simpl_in_cset :=
   | H: (`cset_references_fvar` _ _)   |- _ => go H
   | H: ~ (`cset_references_univ` _ _) |- _ => go H
   | H: (`cset_references_univ` _ _)   |- _ => go H
+  | H: ~ (`cset_references_lvar` _ _) |- _ => go H
+  | H: (`cset_references_lvar` _ _)   |- _ => go H
   end.
 
 Ltac destruct_set_mem_univ bs :=
@@ -445,6 +529,9 @@ Ltac destruct_set_mem a bs :=
   | NatSet.F.t =>
     let H := fresh a "In" in
     destruct (NatSet.F.mem a bs) eqn:H; rewrite_set_facts_in H
+  | LabelSet.F.t =>
+    let H := fresh a "In" in
+    destruct (LabelSet.F.mem a bs) eqn:H; rewrite_set_facts_in H
   | cap =>
     match type of a with
     | atom =>
@@ -460,6 +547,12 @@ Ltac destruct_set_mem a bs :=
     | NatSet.F.elt =>
       let H := fresh a "In" in
       destruct (`cset_references_bvar_dec` a bs) eqn:H; rewrite_set_facts_in H; trivial
+    | label =>
+      let H := fresh a "In" in
+      destruct (`cset_references_lvar_dec` a bs) eqn:H; rewrite_set_facts_in H; trivial
+    | LabelSet.F.elt =>
+      let H := fresh a "In" in
+      destruct (`cset_references_lvar_dec` a bs) eqn:H; rewrite_set_facts_in H; trivial
     end
   end.
 
@@ -468,13 +561,17 @@ Ltac find_and_destroy_set_mem :=
   | H : _ |- context G [`cset_references_fvar_dec` ?X ?S] => destruct_set_mem X S
   | H : _ |- context G [`cset_references_bvar_dec` ?B ?S] => destruct_set_mem B S
   | H : _ |- context G [`cset_references_univ_dec` ?S] => destruct_set_mem_univ S
+  | H : _ |- context G [`cset_references_lvar_dec` ?B ?S] => destruct_set_mem B S
   | H : _ |- context G [AtomSet.F.mem ?X ?S] => destruct_set_mem X S
   | H : _ |- context G [NatSet.F.mem ?N ?S] => destruct_set_mem N S
+  | H : _ |- context G [LabelSet.F.mem ?N ?S] => destruct_set_mem N S
   | H : context G [`cset_references_fvar_dec` ?X ?S] |- _ => destruct_set_mem X S
   | H : context G [`cset_references_bvar_dec` ?B ?S] |- _ => destruct_set_mem B S
   | H : context G [`cset_references_univ_dec` ?S] |- _ => destruct_set_mem_univ S
+  | H : context G [`cset_references_lvar_dec` ?B ?S] |- _ => destruct_set_mem B S
   | H : context G [AtomSet.F.mem ?X ?S] |- _ => destruct_set_mem X S
   | H : context G [NatSet.F.mem ?N ?S] |- _ => destruct_set_mem N S
+  | H : context G [LabelSet.F.mem ?N ?S] |- _ => destruct_set_mem N S
   end.
 
 Lemma funion_empty_idempotent : forall xs, xs `u`N {}N = xs.
@@ -501,11 +598,18 @@ Proof. destr_bool. Qed.
 Lemma or_true_true : forall xs, xs || true = true.
 Proof. destr_bool. Qed.
 
+Lemma lunion_empty_idempotent : forall xs, xs `u`L {}L = xs.
+Proof. intros. lsetdec. Qed.
+
+Lemma empty_lunion_idempotent : forall xs, {}L `u`L xs = xs.
+Proof. intros. lsetdec. Qed.
+
 Hint Rewrite
   funion_empty_idempotent empty_funion_idempotent
   union_empty_idempotent empty_union_idempotent
   or_false_idempotent false_or_idempotent
   true_or_true or_true_true
+  lunion_empty_idempotent empty_lunion_idempotent
 : csets.
 
 Lemma cunion_empty_idempotent : forall xs, xs `u` {} = xs.
@@ -516,9 +620,9 @@ Proof. intros. destruct xs. unfold cset_union. autorewrite with csets; trivial. 
 
 Hint Rewrite cunion_empty_idempotent empty_cunion_idempotent : csets.
 
-Lemma cset_concrete_union : forall xs ns us xs' ns' us',
-  (cset_set xs ns us) `u` (cset_set xs' ns' us') =
-  (cset_set (xs `u`A xs') (ns `u`N ns') (us || us')).
+Lemma cset_concrete_union : forall xs ns us xs' ns' us' ls ls',
+  (cset_set xs ns us ls) `u` (cset_set xs' ns' us' ls') =
+  (cset_set (xs `u`A xs') (ns `u`N ns') (us || us') (ls `u`L ls')).
 Proof. intros. cbv [cset_union]. reflexivity. Qed.
 
 Hint Rewrite cset_concrete_union : csets.
@@ -559,6 +663,7 @@ Ltac csetdec :=
                  try f_equal;
                  try notin_solve; try fsetdec; try solve [exfalso; notin_solve];
                  try nnotin_solve; try fnsetdec; try solve [exfalso; nnotin_solve];
+                 try lnotin_solve; try lsetdec; try solve [exfalso; lnotin_solve];
                  try solve [destr_bool]
                  );
        intuition (csetdec)).
@@ -599,15 +704,15 @@ Proof.
   unfold capt; fnsetdec.
 Qed.
 
-Lemma capt_empty_bvar : forall A N R,
-  capt (cset_set A N R) ->
+Lemma capt_empty_bvar : forall A N R L,
+  capt (cset_set A N R L) ->
   N = {}N.
 Proof.
   intros. unfold capt in *. fnsetdec.
 Qed.
 
-Lemma capt_concrete_cset : forall xs b,
-  capt (cset_set xs {}N b).
+Lemma capt_concrete_cset : forall xs b ls,
+  capt (cset_set xs {}N b ls).
 Proof.
   intros. unfold capt. fnsetdec.
 Qed.
@@ -635,7 +740,7 @@ Lemma subst_over_subset : forall C1 C2 D x,
 Proof.
   intros.
   unfold cset_subset_prop in *.
-  destruct H as [HF [HB HL]].
+  destruct H as [HF [HB [HU HL]]].
   cbv [subst_cset].
   csetdec...
 Qed.
@@ -816,45 +921,47 @@ Lemma open_cset_rec_capt_aux : forall c j V i U,
       and U do not both contain universal*)
   (andb (`cset_uvar` V) (`cset_uvar` U)) = false ->
   AtomSet.F.Empty (AtomSet.F.inter (`cset_fvars` V) (`cset_fvars` U)) ->
+  LabelSet.F.Empty (LabelSet.F.inter (`cset_lvars` V) (`cset_lvars` U)) ->
   open_cset j V c = open_cset i U (open_cset j V c) ->
   c = open_cset i U c.
 Proof with eauto.
-  intros * Hfresh Hempty HdisjointUniv HdisjointV HdisjointL.
+  intros * Hfresh Hempty HdisjointUniv HdisjointV HdisjointL Eq.
   unfold capt, open_cset, cset_union in *.
-  destruct c eqn:Hc; destruct U eqn:HU; destruct V eqn:HV; destruct_set_mem j t0;
-    destruct_set_mem i t0;
-    destruct (NatSet.F.mem i (NatSet.F.union t4 (NatSet.F.remove j t0))) eqn:iInUnion;
-    rewrite_set_facts_in iInUnion; f_equal; autorewrite with csets in *;
-      (* try (repeat destr_bool;autorewrite with csets)...*)
-    inversion HdisjointL; autorewrite with csets;  try fsetdec; try fnsetdec.
-  * assert (t1 `subset` t). {
-      intros e Het1.
-      assert (e `in` (t1 `union` t3 `union` t)) by fsetdec.
-      assert (e `notin` t3) by fsetdec.
-      rewrite <- H0 in H. fsetdec.
+  csetdec; inversion Eq; autorewrite with csets...
+  * assert (t `subset` t5). {
+      intros e Het.
+      assert (e `in` (t `union` t2 `union` t5)) by fsetdec.
+      assert (AtomSet.F.Empty (AtomSet.F.inter t2 t)). {
+        rewrite H. fsetdec.
+      }
+      assert (e `notin` t2) by fsetdec.
+      rewrite <- H1 in H0. fsetdec.
     }
     fsetdec.
-  * assert (NatSet.F.In i (NatSet.F.remove j t0)) by fnsetdec.
-    assert (~NatSet.F.In i (NatSet.F.remove i (NatSet.F.remove j t0))) by fnsetdec.
-    assert (NatSet.F.In i t2). {
-      destruct_set_mem i t2...
-      exfalso.
-      assert (~ NatSet.F.In i (NatSet.F.union t2 (NatSet.F.remove i (NatSet.F.union t4 (NatSet.F.remove j t0)))))
-         by fnsetdec.
-      rewrite <- H1 in H4. fnsetdec.
+  * assert (NatSet.F.In i (NatSet.F.remove j t6)) by fnsetdec.
+    assert (~ NatSet.F.In i (NatSet.F.remove i (NatSet.F.remove j t6))) by fnsetdec.
+    assert (NatSet.F.In i t0). {
+      destruct_set_mem i t0...
+      assert (~ NatSet.F.In i (t0 `u`N (t6 `\`N j) `\`N i)) by
+         fnsetdec.
+      rewrite <- H2 in H6. fnsetdec.
     }
-    assert (NatSet.F.Subset t2 t0). {
-      intros e Het3.
+    assert (NatSet.F.Subset t0 t6). {
+      intros e Het6.
       destruct (e === i); subst...
-      assert (NatSet.F.In e (NatSet.F.union t2 (NatSet.F.remove i (NatSet.F.union t4  (NatSet.F.remove j t0)))))
-        by fnsetdec.
-      rewrite <- H1 in H5...
+      assert (NatSet.F.In e (NatSet.F.union t0 (NatSet.F.remove i (NatSet.F.remove j t6)))). fnsetdec.
+      rewrite <- H2 in H7...
       assert (e <> j) by fnsetdec.
       fnsetdec.
     }
     fnsetdec.
-  * destr_bool...
-  * destr_bool...
+  * assert (t1 `c`L t7). {
+      intros e Het1.
+      assert (e `in`L (t1 `u`L t4 `u`L t7)) by lsetdec.
+      assert (e `~in`L t4) by lsetdec.
+      rewrite <- H4 in H0. lsetdec.
+    }
+    lsetdec.
 Qed.
 
 Lemma subst_cset_open_cset_rec : forall x k C1 C2 D,
@@ -878,90 +985,94 @@ Proof.
 Qed.
 
 
+Lemma atoms_empty_union : forall xs ys,
+  xs `u`A ys = {}A -> xs = {}A /\ ys = {}A.
+Proof with eauto.
+  intros.
+  assert (AtomSet.F.Empty (xs `u`A ys)).
+    rewrite H. fsetdec.
+  split; fsetdec.
+Qed.
+Lemma atoms_empty_union_left : forall xs ys,
+  xs `u`A ys = {}A -> xs = {}A.
+Proof with eauto.
+  intros. apply atoms_empty_union in H as [? ?]...
+Qed.
+Lemma atoms_empty_union_right : forall xs ys,
+  xs `u`A ys = {}A -> ys = {}A.
+Proof with eauto.
+  intros. apply atoms_empty_union in H as [? ?]...
+Qed.
+
+Lemma nats_empty_union : forall xs ys,
+  xs `u`N ys = {}N -> xs = {}N /\ ys = {}N.
+Proof with eauto.
+  intros.
+  assert (NatSet.F.Empty (xs `u`N ys)).
+    rewrite H. fnsetdec.
+  split; fnsetdec.
+Qed.
+Lemma nats_empty_union_left : forall xs ys,
+  xs `u`N ys = {}N -> xs = {}N.
+Proof with eauto.
+  intros. apply nats_empty_union in H as [? ?]...
+Qed.
+Lemma nats_empty_union_right : forall xs ys,
+  xs `u`N ys = {}N -> ys = {}N.
+Proof with eauto.
+  intros. apply nats_empty_union in H as [? ?]...
+Qed.
+
+Lemma univ_empty_union : forall b b',
+  b || b' = false -> b = false /\ b' = false.
+Proof with eauto.
+  intros.
+  destr_bool...
+Qed.
+Lemma univ_empty_union_left : forall b b',
+  b || b' = false -> b = false.
+Proof with eauto.
+  intros. apply univ_empty_union in H as [? ?]...
+Qed.
+Lemma univ_empty_union_right : forall b b',
+  b || b' = false -> b' = false.
+Proof with eauto.
+  intros. apply univ_empty_union in H as [? ?]...
+Qed.
+
+Lemma labels_empty_union : forall xs ys,
+  xs `u`L ys = {}L -> xs = {}L /\ ys = {}L.
+Proof with eauto.
+  intros.
+  assert (LabelSet.F.Empty (xs `u`L ys)).
+    rewrite H. lsetdec.
+  split; lsetdec.
+Qed.
+Lemma labels_empty_union_left : forall xs ys,
+  xs `u`L ys = {}L -> xs = {}L.
+Proof with eauto.
+  intros. apply labels_empty_union in H as [? ?]...
+Qed.
+Lemma labels_empty_union_right : forall xs ys,
+  xs `u`L ys = {}L -> ys = {}L.
+Proof with eauto.
+  intros. apply labels_empty_union in H as [? ?]...
+Qed.
+
+Hint Resolve atoms_empty_union_left atoms_empty_union_right
+              nats_empty_union_left nats_empty_union_right
+              univ_empty_union_left univ_empty_union_right
+              labels_empty_union_left labels_empty_union_right
+  : core.
+
 Lemma empty_cset_union : forall C1 C2,
   cset_union C1 C2 = {} ->
   C1 = {} /\ C2 = {}.
 Proof with eauto.
   intros.
   destruct C1; destruct C2; simpl in H; try discriminate.
-  inversion H.
-  split; f_equal.
-  - destruct (AtomSet.F.choose (t `union` t1)) eqn:Eq.
-    + assert (AtomSet.F.Equal (t `union` t1) {}A) as HA. {
-        rewrite H1.
-        fsetdec.
-      }
-      apply AtomSet.F.choose_1 in Eq.
-      rewrite HA in Eq.
-      exfalso.
-      fsetdec.
-    + apply AtomSet.F.choose_2 in Eq.
-      assert (AtomSet.F.Empty t). {
-        unfold AtomSet.F.Empty in *.
-        unfold not in *.
-        intros.
-        apply (Eq a).
-        fsetdec.
-      }
-      fsetdec.
-  - destruct (NatSet.F.choose (NatSet.F.union t0 t2)) eqn:Eq.
-    + assert (NatSet.F.Equal (NatSet.F.union t0 t2) {}N) as HA. {
-        rewrite H2.
-        fnsetdec.
-      }
-      apply NatSet.F.choose_1 in Eq.
-      rewrite HA in Eq.
-      exfalso.
-      fnsetdec.
-    + apply NatSet.F.choose_2 in Eq.
-      assert (NatSet.F.Empty t0). {
-        unfold NatSet.F.Empty in *.
-        unfold not in *.
-        intros.
-        apply (Eq a).
-        fnsetdec.
-      }
-      fnsetdec.
-  - csetdec.
-  - destruct (AtomSet.F.choose (t `union` t1)) eqn:Eq.
-    + assert (AtomSet.F.Equal (t `union` t1) {}A) as HA. {
-        rewrite H1.
-        fsetdec.
-      }
-      apply AtomSet.F.choose_1 in Eq.
-      rewrite HA in Eq.
-      exfalso.
-      fsetdec.
-    + apply AtomSet.F.choose_2 in Eq.
-      assert (AtomSet.F.Empty t1). {
-        unfold AtomSet.F.Empty in *.
-        unfold not in *.
-        intros.
-        apply (Eq a).
-        fsetdec.
-      }
-      fsetdec.
-  - destruct (NatSet.F.choose (NatSet.F.union t0 t2)) eqn:Eq.
-    + assert (NatSet.F.Equal (NatSet.F.union t0 t2) {}N) as HA. {
-        rewrite H2.
-        fnsetdec.
-      }
-      apply NatSet.F.choose_1 in Eq.
-      rewrite HA in Eq.
-      exfalso.
-      fnsetdec.
-    + apply NatSet.F.choose_2 in Eq.
-      assert (NatSet.F.Empty t2). {
-        unfold NatSet.F.Empty in *.
-        unfold not in *.
-        intros.
-        apply (Eq a).
-        fnsetdec.
-      }
-      fnsetdec.
-  - csetdec.
+  inversion H; split; f_equal; try rewrite H1; try rewrite H2; try rewrite H3; try rewrite H4...
 Qed.
-
 
 Lemma cset_subst_self : forall C x,
   subst_cset x C (`cset_fvar` x) = C.
@@ -996,7 +1107,7 @@ Proof with eauto*.
   unfold cset_union in *.
   destruct C1 eqn:HC1; destruct C2 eqn:HC2; subst...
   inversion Hunion...
-  assert (x `in` (t1 `union` t3)) by (rewrite H1; eauto*)...
+  assert (x `in` (t2 `union` t5)) by (rewrite H1; eauto*)...
   apply AtomSetFacts.union_iff in H0; inversion H0; subst...
 Qed.
 
@@ -1008,18 +1119,7 @@ Proof with eauto.
   intros.
   destruct D1; destruct D2.
   unfold cset_union, subst_cset.
-  destruct_set_mem z t.
-  - assert (AtomSet.F.mem z (t `union` t1) = true) as HA by fset_mem_dec.
-    rewrite HA.
-    unfold cset_union.
-    destruct_set_mem z t1; csetdec.
-  - destruct_set_mem z t1.
-    + assert (AtomSet.F.mem z (t `union` t1) = true) as HA by fset_mem_dec.
-      rewrite HA.
-      unfold cset_union; csetdec.
-    + assert (AtomSet.F.mem z (t `union` t1) = false) as HA by fset_mem_dec.
-      rewrite HA.
-      reflexivity.
+  csetdec.
 Qed.
 
 Lemma notin_cset_fvars_distributive_over_cset_union : forall x C D,
